Regex/Compiler/Patch.lean
@@ -1,6 +1,3 @@
-import Std.Tactic.Do
-import Std.Tactic.Do.Syntax
-
 import Regex.Do.Triple.SpecLemmas
 import Regex.Compiler.Basic
 
@@ -47,8 +44,8 @@ def patch («from» «to» : Unchecked.StateID) : PatchM Unit := do
       set (states.set «from» (Unchecked.State.BackRef b f «to»))
     | .ByteRange t =>
         set (states.set «from» (Unchecked.State.ByteRange {t with «next» := «to»}) h)
-    | .Capture role _ pattern_id group_index slot =>
-        set (states.set «from» (Unchecked.State.Capture role «to» pattern_id group_index slot))
+    | .Capture role _ pattern_id group_index slot isValid =>
+        set (states.set «from» (Unchecked.State.Capture role «to» pattern_id group_index slot isValid))
     | .BinaryUnion alt1 alt2 =>
         if alt1 = 0
         then set (states.set «from» (Unchecked.State.BinaryUnion «to» alt2) h)
@@ -67,14 +64,14 @@ end Code
 
 namespace Lemmas
 
-private theorem all_set_next_of_lt (n : Unchecked.StateID) (s : Unchecked.State)
+theorem all_set_next_of_lt (n : Unchecked.StateID) (s : Unchecked.State)
   (states : Array Unchecked.State)
   (h : n < states.size) (hn : Unchecked.State.nextOf s < states.size)
   (hlt : ∀ (i : Nat) _, states[i].nextOf < states.size)
     : ∀ (i : Nat) (hi : i < states.size), (((states.set n s h)[i]'(by grind)).nextOf < states.size) := by
   grind
 
-private theorem eat_lt («from» s : Nat) (n : Unchecked.StateID) (m : Unchecked.EatMode)
+theorem eat_lt («from» s : Nat) (n : Unchecked.StateID) (m : Unchecked.EatMode)
   (states : Array Unchecked.State) (h : «from» < states.size)
   (hmode : Unchecked.EatMode.nextOf m = s)
   (hm : states[«from»]'h = Unchecked.State.Eat m n)
@@ -85,7 +82,7 @@ private theorem eat_lt («from» s : Nat) (n : Unchecked.StateID) (m : Unchecked
   unfold Unchecked.State.nextOf at hlt
   split at hlt <;> try simp_all [Nat.max_lt]
 
-private theorem change_frame_step_lt («from» : Nat) (f t : Unchecked.StateID)
+theorem change_frame_step_lt («from» : Nat) (f t : Unchecked.StateID)
   (states : Array Unchecked.State) (h : «from» < states.size)
   (hm : states[«from»]'h = Unchecked.State.ChangeFrameStep f t)
   (hlt : states[«from»].nextOf < states.size)
@@ -94,7 +91,7 @@ private theorem change_frame_step_lt («from» : Nat) (f t : Unchecked.StateID)
   unfold Unchecked.State.nextOf at hlt
   grind
 
-private theorem binary_union_lt («from» : Nat) (alt1 alt2 : Unchecked.StateID)
+theorem binary_union_lt («from» : Nat) (alt1 alt2 : Unchecked.StateID)
   (states : Array Unchecked.State) (h : «from» < states.size)
   (hm : states[«from»]'h = Unchecked.State.BinaryUnion alt1 alt2)
   (hlt : states[«from»].nextOf < states.size)
@@ -103,7 +100,7 @@ private theorem binary_union_lt («from» : Nat) (alt1 alt2 : Unchecked.StateID)
   unfold Unchecked.State.nextOf at hlt
   grind
 
-private theorem union_lt («from» to : Nat) (alternates : Array Unchecked.StateID)
+theorem union_lt («from» to : Nat) (alternates : Array Unchecked.StateID)
   (states : Array Unchecked.State) (h : «from» < states.size)
   (ht : to < states.size) (hm : states[«from»]'h = Unchecked.State.Union alternates)
   (hlt : states[«from»].nextOf < states.size)
@@ -112,7 +109,7 @@ private theorem union_lt («from» to : Nat) (alternates : Array Unchecked.State
   simp +zetaDelta [Unchecked.State.nextOf] at hlt
   exact List.maxD_of_append_lt hlt ht
 
-private theorem union_reverse_lt («from» to : Nat) (alternates : Array Unchecked.StateID)
+theorem union_reverse_lt («from» to : Nat) (alternates : Array Unchecked.StateID)
   (states : Array Unchecked.State) (h : «from» < states.size)
   (ht : to < states.size)
   (hm : states[«from»]'h = Unchecked.State.UnionReverse alternates)
@@ -122,37 +119,4 @@ private theorem union_reverse_lt («from» to : Nat) (alternates : Array Uncheck
   simp +zetaDelta [Unchecked.State.nextOf] at hlt
   exact List.maxD_of_append_lt hlt ht
 
-open Std.Do
-
-set_option mvcgen.warning false
-
-@[spec] theorem patch_spec («from»: Unchecked.StateID) {«to» : Unchecked.StateID}
-  {states : Array Unchecked.State}
-    : ⦃fun s => ⌜s = states ∧ nextOfLt states ∧ «from» < states.size ∧ «to» < states.size⌝⦄
-      Code.patch «from» «to»
-      ⦃post⟨fun _ r => ⌜states.size = r.size ∧ «to» < r.size ∧ nextOfLt r⌝, fun _ => ⌜True⌝ ⟩⦄ := by
-  mintro _
-  unfold Code.patch
-  mvcgen
-  all_goals simp_all
-  all_goals try intro _ _; expose_names
-  all_goals try (apply all_set_next_of_lt «from» _ states h_2.right.right.left ?_ (h.right.left)); try assumption
-  all_goals try simp_all [Unchecked.State.nextOf, h_2.right.right.right, Nat.max_lt]
-  all_goals try simp [wp]
-  all_goals try simp [nextOfLt] at h
-  expose_names
-  · simp [eat_lt «from» s_1 n (Unchecked.EatMode.Until s_1)
-      states (by grind) (by simp_all [Unchecked.EatMode.nextOf]) (by simp_all) (by grind)]
-  · simp [eat_lt «from» s_1 n (Unchecked.EatMode.Until s_1)
-      states (by grind) (by simp_all [Unchecked.EatMode.nextOf]) (by simp_all) (by grind)]
-  · simp [eat_lt «from» s_1 n (Unchecked.EatMode.ToLast 0)
-      states (by grind) (by simp_all [Unchecked.EatMode.nextOf]) (by simp_all) (by grind)]
-  · simp [eat_lt «from» s_1 n (Unchecked.EatMode.ToLast s_1)
-      states (by grind) (by simp_all [Unchecked.EatMode.nextOf]) (by simp_all) (by grind)]
-  · simp [change_frame_step_lt «from» f t states (by grind) (by simp_all) (by grind)]
-  · simp [change_frame_step_lt «from» f t states (by grind) (by simp_all) (by grind)]
-  · simp [binary_union_lt «from» alt1 alt2 states (by grind) (by simp_all) (by grind)]
-  · simp [binary_union_lt «from» alt1 alt2 states (by grind) (by simp_all) (by grind)]
-  · simp [union_lt «from» «to» alternates states (by simp_all) (by grind) (by grind) (by grind)]
-  · simp [union_reverse_lt «from» «to» alternates states (by simp_all) (by grind) (by grind) (by grind)]
 end Lemmas
