Regex/Data/Array/Lemmas.lean
@@ -1,7 +1,14 @@
 import Init.Data.List.Lemmas
+import Init.Data.Order.Lemmas
 import Init.Data.Array.Mem
+import Batteries.Data.Array.Basic
+
+import Std.Tactic.Do
+import Std.Tactic.Do.Syntax
 
 import Regex.Data.List.Lemmas
+import Regex.Data.Ord.Basic
+import Regex.Data.Nat.Basic
 import Regex.Data.Array.Basic
 
 namespace Array
@@ -118,3 +125,297 @@ theorem concat_of_pop? {arr : Array α} (h : Array.pop? arr = some (last, arr'))
 theorem get_eq_get?_some {as : Array α} (hlt : i < as.size) (h : a = as[i]'hlt)
     : as[i]? = some a := by
   simp_all
+
+@[simp] theorem size_of_head?_lt (as : Array α) (h : as.toList.head? = some a) : 0 < as.size := by
+  unfold Array.size
+  unfold List.head? at h
+  split at h <;> simp_all
+
+private theorem unique.acc_mem_snd [DecidableEq α]
+    : ∀ (acc : (α × Array α)) (r : α), 0 < acc.snd.size
+      → acc.fst ∈ acc.snd
+      → (unique.acc acc r).snd.toList.head? = acc.snd.toList.head?
+        ∧ (unique.acc acc r).fst ∈ (unique.acc acc r).snd.toList
+        ∧ ∀ a ∈ acc.snd, a ∈ (unique.acc acc r).snd
+        ∧ r ∈ (unique.acc acc r).snd := by
+    unfold unique.acc
+    have (x : (α × Array α)) (r : α) : (if x.fst = r then (r, x.snd) else (r, x.snd.push r))
+        = (if x.fst = r then (r, x.snd) else (r, x.snd ++ #[r])) := by
+      rfl
+    intros
+    and_intros
+    · simp [List.head?]; split <;> rename_i heq <;> split at heq <;> split <;> simp_all
+    all_goals simp_all <;> split <;> simp_all
+
+private theorem unique.mem_foldl [DecidableEq α]
+  (l : List α) (a head : α) (init : α × Array α) (ha : a ∈ l || a ∈ init.snd.toList)
+  (hi1 : init.snd.toList.head? = some head) (hi2 : init.fst ∈ init.snd)
+    : a ∈ (List.foldl unique.acc init l).snd := by
+  have hf := @unique.acc_mem_snd α
+  induction l generalizing init with
+  | nil =>
+    simp_all
+  | cons a' l ih =>
+    simp at ih
+    simp [List.foldl_cons]
+    expose_names
+    simp at ha
+    cases ha
+    · rename_i ha
+      cases ha
+      · have := @ih (unique.acc init a').fst (unique.acc init a').snd
+            (by exact Or.inr (by have := hf init a' (by simp_all) (by grind); grind))
+            (by have := hf init a (by simp_all) (by grind); grind)
+            (by grind)
+        simp_all
+      · have := @ih (unique.acc init a').fst (unique.acc init a').snd
+            (by exact Or.inl (by simp_all))
+            (by have := hf init a (by simp_all) (by grind); grind)
+            (by grind)
+        simp_all
+    · expose_names
+      have := @ih (unique.acc init a').fst (unique.acc init a').snd
+            (by exact Or.inr (by have := hf init a' (by simp_all); grind))
+            (by have := hf init a (by simp_all) (by grind); grind)
+            (by grind)
+      simp_all
+
+private theorem unique.mem_of_foldl [DecidableEq α]
+  (l : List α) (a : α) (init : α × Array α) (ha1 : a ∈ (List.foldl unique.acc init l).snd)
+  (ha2 : ¬a ∈ init.snd) (hne : ¬l = [])
+    : a ∈ l := by
+  induction l generalizing init with
+  | nil => contradiction
+  | cons a' l ih =>
+    by_cases a = a'
+    · grind
+    · simp [List.foldl_cons] at ha1
+      by_cases h : a ∈ (unique.acc init a').snd
+      · have hf : ∀ a a' (acc : α × Array α), a ∈ (unique.acc acc a').snd → a ∈ acc.snd ∨ a ∈ acc.snd ++ #[a'] := by
+          intro a a acc h
+          unfold unique.acc at h
+          grind
+        have := hf a a' init h
+        simp_all
+      · by_cases l = []
+        · simp_all
+        · have := ih (unique.acc init a') ha1 (by grind) (by grind)
+          simp_all
+
+protected theorem unique.mem_of_mem_unqiue [DecidableEq α] [LE α] (as : Array α)
+    : a ∈ as.unique → a ∈ as := by
+  simp [Array.unique]
+  split
+  · grind
+  · grind
+  · expose_names
+    generalize hi : (head, #[head]) = init
+    by_cases a = head
+    · intro ha
+      apply Array.mem_toList_iff.mp
+      grind
+    · intro ha
+      have := unique.mem_of_foldl tail a init ha (by grind)
+      apply Array.mem_toList_iff.mp
+      simp_all
+
+private theorem unique.mem_unique_of_mem [DecidableEq α] [LE α] (as : Array α)
+  : a ∈ as → a ∈ as.unique := by
+  simp [Array.unique]
+  cases as
+  rename_i l
+  split
+  · simp_all
+  · simp_all
+  · intro ha
+    expose_names
+    generalize hi : (head, #[head]) = init
+    have hi : init.snd.toList.head? = some head := by rw [← hi]; simp [List.head?]
+    simp at heq
+    simp at ha
+    rw [heq] at ha
+    cases ha
+    · unfold List.head? at hi
+      split at hi
+      · grind
+      · expose_names
+        exact unique.mem_foldl tail a a init
+              (by simp_all) (by unfold List.head?; split <;> grind) (by grind)
+    · exact unique.mem_foldl tail a head init
+              (by simp_all; expose_names; exact Or.symm (Or.inr h_1)) (by grind)  (by grind)
+
+@[simp] theorem mem_unique [DecidableEq α] [LE α] (as : Array α) : a ∈ as.unique ↔ a ∈ as :=
+  ⟨by intro h; exact unique.mem_of_mem_unqiue as h, by intro h; exact unique.mem_unique_of_mem as h⟩
+
+private theorem nodup.nodup_acc_if_nodup [DecidableEq α] [LE α] [LT α] [Std.IsPreorder α]
+  [Std.LawfulOrderLT α] [Std.Antisymm fun (x1 x2 : α) => x1 ≤ x2]
+    : ∀ a (acc : α × Array α), acc.fst ≤ a → (∀ a' ∈ acc.snd.toList, a' ≤ acc.fst)
+        → acc.snd.toList.Nodup → (unique.acc acc a).snd.toList.Nodup := by
+  intros
+  expose_names
+  unfold List.Nodup at h_2
+  unfold List.Nodup unique.acc
+  split
+  assumption
+  simp_all
+  apply List.pairwise_append.mpr
+  have := @Std.LawfulOrderLT.lt_iff α _ _ _ -- for grind
+  have : ∀ (a b c : α), a ≤ b ∧ b ≤ c ∧ ¬b = c → a < c := by -- for grind
+    intro a b c h
+    exact Std.lt_of_le_of_lt h.left (Std.lt_of_le_of_ne h.right.left h.right.right)
+  and_intros <;> grind
+
+private theorem nodup.nodup_of_foldl [DecidableEq α] [LE α] [LT α] [Std.IsPreorder α]
+  [Std.LawfulOrderLT α] [Std.Antisymm fun (x1 x2 : α) => x1 ≤ x2]
+  (l : List α) (init : α × Array α)
+  (h : l.Pairwise LE.le)
+  (ha1 : (∀ (a' : α), a' ∈ init.snd.toList → a' ≤ init.fst))
+  (ha2 : init.snd.toList.Nodup)
+  (ha3 : (∀ (a : α), a ∈ l → init.fst ≤ a))
+    : (List.foldl unique.acc init l).snd.toList.Nodup := by
+  have := @Std.IsPreorder.le_trans α _ _ -- for grind
+  have := @Std.IsPreorder.le_refl α -- for grind
+  have := @nodup_acc_if_nodup α
+  have : ∀ a a' (acc : α × Array α), acc.fst ≤ a → (∀ a' ∈ acc.snd.toList, a' ≤ acc.fst)
+         → a' ∈ (unique.acc acc a).snd → a' ≤ (unique.acc acc a).fst := by
+    intro _ _ _ _ _ h
+    unfold unique.acc at h
+    unfold unique.acc
+    split <;> grind
+  have : ∀ a (acc : α × Array α), (unique.acc acc a).fst ≤ a := by unfold unique.acc; grind
+  induction l generalizing init with
+  | nil => simp_all
+  | cons a l ih =>
+    simp [List.foldl_cons]
+    expose_names
+    by_cases l = []
+    · simp_all
+    · expose_names
+      have ih := ih (unique.acc init a) (by grind) (by simp_all) (by grind) (by
+        intros
+        simp_all
+        grind)
+      simp_all
+
+@[simp] theorem nodup_unique [DecidableEq α] [LE α] [LT α] [Std.IsPreorder α]
+  [Std.LawfulOrderLT α] [Std.Antisymm fun (x1 x2 : α) => x1 ≤ x2] (as : Array α)
+  (h : as.toList.Pairwise LE.le)
+    : List.Nodup as.unique.toList := by
+  have := @Std.IsPreorder.le_trans α _ _ -- for grind
+  have := @Std.IsPreorder.le_refl α -- for grind
+  simp [Array.unique]
+  cases as
+  rename_i l
+  split
+  · simp_all
+  · simp_all
+  · expose_names
+    generalize hi : (head, #[head]) = init
+    have : ∀ (a : α), a ∈ tail → init.fst ≤ a := by rw [← hi]; simp_all
+    apply nodup.nodup_of_foldl tail init
+    all_goals grind
+
+@[simp] theorem mergeSort_toList_eq (as bs: Array α) (le : α → α → Bool := by exact fun a b => a ≤ b)
+  (h : bs = as.mergeSort le) : as.toList.mergeSort le = bs.toList := by
+  unfold Array.mergeSort at h
+  grind
+
+@[simp] theorem mem_mergeSort [LT α] (as : Array α) (le : α → α → Bool := by exact (· ≤ ·))
+    : a ∈ as.mergeSort le ↔ a ∈ as := by
+  unfold Array.mergeSort
+  simp_all only [mem_toArray, List.mem_mergeSort, mem_toList_iff]
+
+open Std.Do
+
+theorem minWith_spec [ord : Ord α] [Std.TransOrd α] (as : Array α) (init : α)
+  (f : α → α → α) (hf : (fun min x => if @compare α ord x min = Ordering.lt then x else min) = f)
+  (lt_iff : ∀ a b : α, (Ord.toLT ord).lt a b ↔ (Ord.toLE ord).le a b ∧ ¬ (Ord.toLE ord).le b a)
+  (le_notLt : ∀ a b : α, ¬(Ord.toLT ord).lt a b ↔ (Ord.toLE ord).le b a)
+    : ⦃⌜True⌝⦄
+      (Array.foldlM f init as : Id α)
+      ⦃⇓r => ⌜(Ord.toLE ord).le r init ∧ ∀ a ∈ as, (Ord.toLE ord).le r a⌝⦄ := by
+  have le_refl : ∀ a : α, (Ord.toLE ord).le a a := by grind
+  have le_trans : ∀ a b c : α, letI le := (Ord.toLE ord).le; le a b → le b c → le a c := by
+    apply Std.TransOrd.isLE_trans
+  mintro _
+  mspec Spec.foldlM_array
+  case inv => exact (⇓ (xs, r) => ⌜(Ord.toLE ord).le r init
+                                    ∧ ∀ a ∈ xs.prefix, (Ord.toLE ord).le r a⌝)
+  case pre => simp_all
+  case post.success => simp_all
+  case step =>
+    simp_all
+    intro pref curr suff h r
+    mintro _
+    simp_all
+    intro hb ha
+    rw [← hf]
+    simp_all
+    split
+    · simp [wp, Id.run]
+      and_intros
+      · expose_names
+        have : @LT.lt α ltOfOrd curr r := by assumption
+        have := (lt_iff curr r).mp (by grind)
+        grind
+      · expose_names
+        intro a ha
+        cases ha
+        · expose_names
+          have : @LT.lt α ltOfOrd curr r := by assumption
+          have := (lt_iff curr r).mp (by grind)
+          have ha := ha a h_2
+          grind
+        · grind
+    · simp [wp, Id.run]
+      and_intros
+      · grind
+      · intro a ha
+        cases ha
+        · expose_names
+          exact le_trans r r a (by grind) (ha a h_2)
+        · expose_names
+          have : (Ord.toLE ord).le r curr := by
+            have h : ¬@LT.lt α ltOfOrd curr r := by assumption
+            have h := le_notLt curr r
+            cases h <;> simp_all
+          grind
+
+theorem min_le_mem [ord : Ord α] [Std.TransOrd α]
+  (xs : Array α) (h : xs.min? = some m)
+  (lt_iff : ∀ a b : α, (Ord.toLT ord).lt a b ↔ (Ord.toLE ord).le a b ∧ ¬ (Ord.toLE ord).le b a)
+  (le_notLt : ∀ a b : α, ¬(Ord.toLT ord).lt a b ↔ (Ord.toLE ord).le b a)
+    : ∀ a ∈ xs, (Ord.toLE ord).le m a := by
+  unfold Array.min? Array.minD Array.minWith at h
+  split at h
+  · simp at h
+    generalize hf : (fun min x => if @compare α ord x min = Ordering.lt then x else min) = f at h
+    unfold Array.foldl at h
+    let xs' := xs.extract 1 xs.size
+    have hex : xs' = xs.extract 1 := by simp +zetaDelta
+    have heq := (minWith_spec xs' xs[0] f hf (by grind) (by grind)) (by simp_all)
+    simp [wp] at heq
+    have hm : foldl (fun x1 x2 => Id.run (f x1 x2)) xs[0] xs' = m := by
+      simp [Id.run, pure] at h
+      simp [Id.run]
+      rw [hex, ← h]
+      exact id (Eq.symm (@Array.foldlM_start_stop α α Id Id.instMonad xs f xs[0] 1 xs.size))
+    intro a ha
+    by_cases h: a = xs[0]
+    · have heq := heq.left
+      rwa [hm, ← h] at heq
+    · have heq := heq.right a (by
+        rw [hex]
+        apply Array.mem_extract_iff_getElem.mpr
+        have ⟨i, ⟨hi, hmem⟩⟩ := Array.mem_iff_getElem.mp ha
+        exact ⟨i-1, by grind⟩)
+      rwa [hm] at heq
+  · simp_all
+
+theorem mem_le_max [ord : Ord α] [Std.TransOrd α] (xs : Array α)
+  (h : xs.max? = some m)
+  (lt_iff : ∀ a b : α, (Ord.toLT ord).lt a b ↔ (Ord.toLE ord).le a b ∧ ¬ (Ord.toLE ord).le b a)
+  (le_iff : ∀ a b : α, ¬(Ord.toLT ord).lt a b ↔ (Ord.toLE ord).le b a)
+    : ∀ a ∈ xs, (Ord.toLE ord).le a m := by
+  unfold Array.max? at h
+  exact @min_le_mem α m ord.opposite _ xs h (by simp_all) (by intro a b; exact le_iff b a)
