Regex/Data/Ord/Basic.lean
@@ -1,0 +1,23 @@
+namespace Ord
+
+theorem toLE_opposite_eq [ord : Ord α] : ∀ (a b : α),
+    (Ord.toLE ord.opposite).le a b ↔ (Ord.toLE ord).le b a  := by
+  unfold Ord.toLE leOfOrd
+  intro a b
+  rw [iff_def]
+  and_intros <;> intro h <;> assumption
+
+theorem toLT_opposite_eq [ord : Ord α] : ∀ (a b : α),
+    (Ord.toLT ord.opposite).lt a b ↔ (Ord.toLT ord).lt b a  := by
+  unfold Ord.toLT ltOfOrd
+  intro a b
+  rw [iff_def]
+  and_intros <;> intro h <;> assumption
+
+@[simp] theorem toLT_iff_opposite [ord : Ord α]
+  (lt_iff : ∀ a b : α, (Ord.toLT ord).lt a b ↔ (Ord.toLE ord).le a b ∧ ¬ (Ord.toLE ord).le b a)
+    : ∀ (a b : α), (Ord.toLT ord.opposite).lt a b
+    ↔ (Ord.toLE ord.opposite).le a b ∧ ¬(Ord.toLE ord.opposite).le b a  := by
+  intro a b
+  rw [toLT_opposite_eq a b, toLE_opposite_eq b a]
+  exact lt_iff b a
