Regex/NFA/Basic.lean
@@ -1,0 +1,562 @@
+import Batteries.Data.Fin.Basic
+import Regex.Utils
+import Regex.Data.List.Lemmas
+import Regex.Data.Array.Basic
+
+namespace NFA
+
+/-- The identifier of a regex pattern, represented by a Nat -/
+abbrev PatternID := Nat
+
+namespace Capture
+
+inductive Role where
+  | Start
+  | End
+deriving BEq, DecidableEq
+
+instance : LawfulBEq Role where
+  eq_of_beq {a b} h := by cases a <;> cases b <;> first | rfl | contradiction
+  rfl {a} := by cases a <;> decide
+
+instance  : ReflBEq Role where
+  rfl {r} := beq_self_eq_true' r.toCtorIdx
+
+@[simp] def toSlot (role : Role) (group : Nat) :=
+  match role with
+  | .Start => group * 2
+  | .End => group * 2 + 1
+
+@[simp] def IsValid (role : Role) (group slot : Nat) :=
+  match role with
+  | .Start => group * 2 = slot
+  | .End => group * 2 + 1 = slot
+
+def toString : Role -> String
+  | .Start => s!"Start"
+  | .End => s!"End"
+
+instance : ToString Role where
+  toString := toString
+
+end Capture
+
+/-- A capture location.
+  `slot` in this context refers to the specific capture group slot
+    offset that is being recorded. Each capturing group has two slots
+    corresponding to the start and end of the matching portion of that
+    group. -/
+@[ext] structure Capture where
+  role: Capture.Role
+  group : Nat
+  slot: Nat
+  isValid : Capture.IsValid role group slot
+
+namespace Capture
+
+abbrev SlotGroup := Nat × Nat
+
+/-- Transform `captures` to a sorted array of (slot, group) tuples. -/
+def toSlots (captures : Array NFA.Capture) : Array SlotGroup :=
+  let slots := captures.map f
+  Array.mergeSort slots le |> Array.unique
+where
+  f c := (c.slot, c.group)
+  le := fun (a : SlotGroup) (b : SlotGroup) => decide (a.1 ≤ b.1)
+
+/-- A valid capture array consists of capture groups with two slots.
+  For every capture group slot with `Role.End` exists a group slot with `Role.Start` -/
+@[simp] def valid (captures : Array NFA.Capture) :=
+    (∀ c : { c : NFA.Capture // c ∈ captures ∧ c.slot % 2 = 0 },
+            c.val.role = Capture.Role.Start ∧ c.val.slot = c.val.group * 2)
+    ∧ (∀ c : { c : NFA.Capture // c ∈ captures ∧ c.slot % 2 = 1 },
+            c.val.role = Capture.Role.End ∧ c.val.slot = c.val.group * 2 + 1)
+    ∧ ∀ c : { c : NFA.Capture // c ∈ captures ∧ c.role = Capture.Role.End },
+      (∃ c' ∈ captures, c'.role = Capture.Role.Start ∧ c.val.group = c'.group)
+
+end Capture
+
+namespace Slots
+
+/-- A valid slot array of (slot, group) tuples consists of groups with two slots
+    at consecutive positions. The groups are not always consecutive,
+    i.e. regex '(a){0}(a)' with slots #[(0, 0), (1, 0), (4, 2), (5, 2)] -/
+@[simp] def Valid (slots : Array Capture.SlotGroup) :=
+  (∀ slot : { slot : Capture.SlotGroup // slot ∈ slots ∧ slot.1 % 2 = 0 }, slot.val.1 = slot.val.2 * 2)
+  ∧ (∀ slot : { slot : Capture.SlotGroup // slot ∈ slots ∧ slot.1 % 2 = 1 }, slot.val.1 = slot.val.2 * 2 + 1)
+  ∧ (∀ slot : { slot : Capture.SlotGroup // slot ∈ slots ∧ slot.1 = slot.2 * 2 + 1 },
+    ∃ slot' ∈ slots, (slot.val.2 = slot'.2 ∧ slot'.1 = slot'.2 * 2))
+
+end Slots
+
+/-- The high-level intermediate representation for a look-around assertion. -/
+inductive Look where
+  /-- Match the beginning of text. -/
+  | Start : Look
+  /-- Match the end of text. -/
+  | End : Look
+  /-- Match the end of text (before optional newline). -/
+  | EndWithOptionalLF : Look
+  /-- Match the beginning of a line or the beginning of text. -/
+  | StartLF : Look
+  /-- Match of a line or the end of text. -/
+  | EndLF : Look
+  /-- Match the beginning of a line or the beginning of text. -/
+  | StartCRLF : Look
+  /-- Match of a line or the end of text. -/
+  | EndCRLF : Look
+  /-- Match a Unicode-aware word boundary. -/
+  | WordUnicode : Look
+  /-- Match a Unicode-aware negation of a word boundary. -/
+  | WordUnicodeNegate : Look
+  /-- Match the start of a Unicode word boundary. -/
+  | WordStartUnicode : Look
+  /-- Match the end of a Unicode word boundary. -/
+  | WordEndUnicode : Look
+  /-- Match the start half of a Unicode word boundary. -/
+  | WordStartHalfUnicode : Look
+  /-- Match the end half of a Unicode word boundary. -/
+  | WordEndHalfUnicode : Look
+  /-- Match the end of the previous match or start of string -/
+  | PreviousMatch : Look
+  /-- Clear matches -/
+  | ClearMatches : Look
+deriving BEq, DecidableEq
+
+namespace Look
+
+def toString : Look -> String
+  | .Start => s!"Start"
+  | .End => s!"End"
+  | .EndWithOptionalLF => s!"EndWithOptionalLF"
+  | .StartLF => s!"StartLF"
+  | .EndLF => s!"EndLF"
+  | .StartCRLF => s!"StartCRLF"
+  | .EndCRLF => s!"EndCRLF"
+  | .WordUnicode => s!"WordUnicode"
+  | .WordUnicodeNegate => s!"WordUnicodeNegate"
+  | .WordStartUnicode => s!"WordStartUnicode"
+  | .WordEndUnicode => s!"WordEndUnicode"
+  | .WordStartHalfUnicode => s!"WordStartHalfUnicode"
+  | .WordEndHalfUnicode => s!"WordEndHalfUnicode"
+  | .PreviousMatch => s!"PreviousMatch"
+  | .ClearMatches => s!"ClearMatches"
+
+end Look
+
+instance : ToString Look where
+  toString := Look.toString
+
+namespace Unchecked
+
+/-- The identifier of a finite automaton state, represented by a Nat.
+    The identifier may refer to a non existing state. -/
+abbrev StateID := Nat
+
+inductive EatMode where
+  /-- Eat frames until State  found -/
+  | Until : StateID -> EatMode
+  /-- Eat frames inclusive last occurunce of State. -/
+  | ToLast : StateID -> EatMode
+deriving BEq, DecidableEq
+
+namespace EatMode
+
+def toString : EatMode -> String
+  | .Until sid => s!"Until {sid}"
+  | .ToLast sid => s!"ToLast {sid}"
+
+@[grind] def nextOf (m : EatMode) : Nat :=
+  match m with
+  |.Until next => next
+  |.ToLast next => next
+
+end EatMode
+
+instance : ToString EatMode where
+  toString := EatMode.toString
+
+/-- A single transition to another state.
+    This transition may only be followed if the current char in the haystack
+    falls in the inclusive range of chars specified. -/
+structure Transition where
+  /-- The inclusive start of the char range. -/
+  start: UInt32
+  /-- The inclusive end of the char range. -/
+  «end»: UInt32
+  /--  The identifier of the state to transition to. -/
+  next: StateID
+deriving BEq, DecidableEq
+
+namespace Transition
+
+/-- check if `c` falls in the inclusive range of chars specified in Transition `trans` -/
+def «matches» (trans : Transition) (c : Char) : Bool :=
+  trans.start <= c.val && c.val <= trans.end
+
+end Transition
+
+/-- A state in an NFA. -/
+inductive State where
+  /-- An empty state whose only purpose is to forward the automaton to
+      another state via an unconditional epsilon transition. -/
+  | Empty (next: StateID) : State
+  /-- use next char -/
+  | NextChar (offset : Nat) (next: StateID) : State
+  /-- Fail, force backtrack -/
+  | Fail : State
+  /-- remove Frame.Step in stack  -/
+  | Eat (mode : EatMode) (next: StateID) : State
+  /-- change Frame.Step in stack and force backtrack -/
+  | ChangeFrameStep («from» to: StateID) : State
+  /-- remove Frame.Step in stack and force backtrack -/
+  | RemoveFrameStep (sid : StateID) : State
+  /--  A state with a single transition may only be followed if the currunt chars match the
+    backrefence to the capturung group. -/
+  | BackRef (n : Nat) (case_insensitive : Bool) (sid : StateID) : State
+  /-- A state with a single transition that can only be taken if the current
+      input symbol is in a particular range of chars. -/
+  | ByteRange (trans : Transition) : State
+  /-- A sequence of transitions used to represent a sparse state. -/
+  | SparseTransitions (transitions : Array Transition) : State
+  /-- A conditional epsilon transition satisfied via some sort of look-around.  -/
+  | Look (look : Look) (next: StateID) : State
+  /--An alternation such that there exists an epsilon transition to all states in `alternates`,
+     where matches found via earlier transitions are preferred over later transitions. -/
+  | Union (alternates: Array StateID) : State
+  /--An alternation such that there exists an epsilon transition to all states in `alternates`,
+     where matches found via later transitions are preferred over earlier transitions. -/
+  | UnionReverse (alternates: Array StateID) : State
+  /-- An alternation such that there exists precisely two unconditional epsilon transitions -/
+  | BinaryUnion (alt1: StateID) (alt2: StateID) : State
+  /-- An empty state that records a capture location.
+      `slot` in this context refers to the specific capture group slot
+       offset that is being recorded. Each capturing group has two slots
+       corresponding to the start and end of the matching portion of that
+       group. -/
+  | Capture (role : Capture.Role) (next: StateID) (pattern_id: PatternID) (group : Nat)
+    (slot: Nat) (isValid : Capture.IsValid role group slot) : State
+  /-- A match state. There is at least one such occurrence of this state for
+      each regex that can match that is in this NFA. -/
+  | Match (pattern_id : PatternID) : State
+deriving BEq, DecidableEq
+
+private def beq' :  State → State → Bool
+  | .Empty n1 , .Empty n2  => n1 = n2
+  | .ByteRange trans1 , .ByteRange trans2  =>
+      trans1.start = trans2.start && trans1.«end» = trans2.«end» && trans1.next = trans2.next
+  | .SparseTransitions trans1 , .SparseTransitions trans2 => trans1.size = trans2.size
+  | .Capture r1 n1 _ g1 s1 _,  .Capture r2 n2 _ g2 s2 _ => r1 == r2 && n1 = n2 && g1 = g2 && s1 = s2
+  | .Match p1,  .Match p2 => p1 = p2
+  | _, _ => false
+
+instance : BEq State where
+  beq := beq'
+
+namespace State
+
+def toString : State -> String
+  | .Empty next => s!"State.Empty => {next}"
+  | .NextChar offset next => s!"State.NextChar offset  {offset} => {next}"
+  | .Fail => s!"State.Fail"
+  | .Eat s n => s!"State.Eat {s} => {n}"
+  | .ChangeFrameStep «from» to => s!"State.ChangeFrameStep from {«from»} to {to}"
+  | .RemoveFrameStep sid => s!"State.RemoveFrameStep {sid}"
+  | .BackRef b f sid =>
+      s!"State.BackRef {b} {if f then "case_insensitive" else ""} => {sid}"
+  | .ByteRange trans =>
+      s!"State.ByteRange {UInt32.intAsString trans.start}-{UInt32.intAsString trans.end} => {trans.next}"
+  | .SparseTransitions trans =>
+      let lines := String.join (trans.toList |> List.map (fun t =>
+            s!" {UInt32.intAsString t.start}-{UInt32.intAsString t.end} => {t.next}"))
+      s!"State.SparseTransitions [{lines} ]"
+  | .Look look next =>
+      s!"State.Look {look} => {next}"
+  | .Union alts =>
+      let lines := String.join (alts.toList |> List.map (fun t => s!" {t}"))
+      s!"State.Union [{lines} ]"
+  | .UnionReverse alts =>
+      let lines := String.join (alts.toList |> List.map (fun t => s!" {t}"))
+      s!"State.UnionReverse [{lines} ]"
+  | .BinaryUnion alt1 alt2 => s!"State.BinaryUnion({alt1}, {alt2})"
+  | .Capture role next pattern_id group slot _ =>
+      s!"State.Capture {role}(pid={pattern_id}, group={group}, slot={slot}) => {next}"
+  | .Match pattern_id => s!"State.Match ({pattern_id})"
+
+/-- next StateID of State `s` -/
+@[grind] def nextOf (s : State) : StateID :=
+  match s with
+  | .Empty next => next
+  | .NextChar _ next => next
+  | .Fail => 0
+  | .Eat (EatMode.Until s) next => Nat.max s next
+  | .Eat (EatMode.ToLast s) next => Nat.max s next
+  | .ChangeFrameStep f t => Nat.max f t
+  | .RemoveFrameStep next => next
+  | .BackRef _ _ next => next
+  | .ByteRange trans => trans.next
+  | .SparseTransitions trans => (trans.map (·.next)).toList.maxD 0
+  | .Look _ next => next
+  | .Union alts => alts.toList.maxD 0
+  | .UnionReverse alts => alts.toList.maxD 0
+  | .BinaryUnion alt1 alt2 => Nat.max alt1 alt2
+  | .Capture _ next _ _ _ _ => next
+  | .Match _ => 0
+
+end State
+
+instance : ToString State where
+  toString := State.toString
+
+/-- A char oriented Thompson non-deterministic finite automaton (NFA). -/
+structure NFA where
+  states : Array State
+  start_anchored: StateID
+  start_unanchored: StateID
+
+namespace NFA
+
+def toString (nfa : NFA) : String :=
+  let states := Array.mapFinIdx nfa.states (fun i s _ => (i, s))
+  let states := String.join (states.toList |> List.map (fun (i, s) =>
+      let iv := String.mk (Nat.toDigits 10 i)
+      "\n  " ++ iv ++ ": " ++ s.toString))
+  s!"states {states}"
+
+end NFA
+
+end Unchecked
+
+instance : ToString Unchecked.NFA where
+  toString := Unchecked.NFA.toString
+
+namespace Checked
+
+inductive EatMode n where
+  /-- Eat frames until State  found -/
+  | Until : Fin n -> EatMode n
+  /-- Eat frames inclusive last occurunce of State. -/
+  | ToLast : Fin n -> EatMode n
+deriving BEq, DecidableEq
+
+namespace EatMode
+
+def toString : EatMode n -> String
+  | .Until sid => s!"Until {sid}"
+  | .ToLast sid => s!"ToLast {sid}"
+
+end EatMode
+
+instance : ToString (EatMode n) where
+  toString := EatMode.toString
+
+/-- A single transition to another state.
+    This transition may only be followed if the current char in the haystack
+    falls in the inclusive range of chars specified. -/
+structure Transition (n : Nat) where
+  /-- The inclusive start of the char range. -/
+  start: Nat
+  /-- The inclusive end of the char range. -/
+  «end»: Nat
+  /--  The identifier of the state to transition to. -/
+  next: Fin n
+deriving BEq, DecidableEq
+
+namespace Transition
+
+/-- check if `c` falls in the inclusive range of chars specified in Transition `trans` -/
+def «matches» (trans : Transition n) (c : Char) : Bool :=
+  trans.start <= c.val.toFin && c.val.toFin <= trans.end
+
+end Transition
+
+/-- A state in an NFA, the elements of `Fin n` refer to existing states in the NFA. -/
+inductive State (n : Nat) where
+  /-- An empty state whose only purpose is to forward the automaton to
+      another state via an unconditional epsilon transition. -/
+  | Empty (next: Fin n) : State n
+  /-- use netx char -/
+  | NextChar (offset : Nat) (next: Fin n) : State n
+  /-- Fail, force backtracking -/
+  | Fail : State n
+  /-- remove Frame.Step in stack  -/
+  | Eat (mode : EatMode n) (next: Fin n) : State n
+  /-- change Frame.Step in stack and force backtracking -/
+  | ChangeFrameStep (fr to: Fin n) : State n
+  /-- remove Frame.Step in stack and force backtrack -/
+  | RemoveFrameStep (sid : Fin n) : State n
+  /--  A state with a single transition may only be followed if the current chars match the
+      backrefence to the capturung group. -/
+  | BackRef (b : Nat) (case_insensitive : Bool) (sid : Fin n) : State n
+  /-- A state with a single transition that can only be taken if the current
+      input symbol is in a particular range of chars. -/
+  | ByteRange (trans : Transition n) : State n
+  /-- A sequence of transitions used to represent a sparse state. -/
+  | SparseTransitions (transitions : Array $ Transition n) : State n
+  /-- A conditional epsilon transition satisfied via some sort of look-around.  -/
+  | Look (look : Look) (next: Fin n) : State n
+  /--An alternation such that there exists an epsilon transition to all states in `alternates`,
+     where matches found via earlier transitions are preferred over later transitions. -/
+  | Union (alternates: Array $ Fin n) : State n
+  /--An alternation such that there exists an epsilon transition to all states in `alternates`,
+     where matches found via later transitions are preferred over earlier transitions. -/
+  | UnionReverse (alternates: Array $ Fin n) : State n
+  /-- An alternation such that there exists precisely two unconditional epsilon transitions -/
+  | BinaryUnion (alt1: Fin n) (alt2: Fin n) : State n
+  /-- An empty state that records a capture location.
+      `slot` in this context refers to the specific capture group slot
+       offset that is being recorded. Each capturing group has two slots
+       corresponding to the start and end of the matching portion of that
+       group. -/
+  | Capture (role: Capture.Role) (next: Fin n) (pattern_id: PatternID) (group : Nat)
+      (slot: Nat) (isValid : Capture.IsValid role group slot) : State n
+  /-- A match state. There is at least one such occurrence of this state for
+      each regex that can match that is in this NFA. -/
+  | Match (pattern_id : PatternID) : State n
+deriving BEq, DecidableEq
+
+private def beq' :  State n → State n → Bool
+  | .Empty ⟨n1, _⟩ , .Empty ⟨n2, _⟩  => n1 = n2
+  | .ByteRange trans1 , .ByteRange trans2  =>
+      trans1.start = trans2.start && trans1.«end» = trans2.«end» && trans1.next = trans2.next
+  | .SparseTransitions trans1 , .SparseTransitions trans2 => trans1.size = trans2.size
+  | .Capture r1 ⟨n1, _⟩ _ g1 s1 _,  .Capture r2 ⟨n2, _⟩ _ g2 s2 _ => r1 == r2 && n1 = n2 && g1 = g2 && s1 = s2
+  | .Match p1,  .Match p2 => p1 = p2
+  | _, _ => false
+
+instance : BEq (State n) where
+  beq := beq'
+
+namespace State
+
+def toString : State n -> String
+  | .Empty next => s!"State.Empty => {next}"
+  | .NextChar offset next => s!"State.NextChar offset {offset} => {next}"
+  | .Fail => s!"State.Fail"
+  | .Eat s next => s!"State.Eat {s} => {next}"
+  | .ChangeFrameStep f t => s!"State.ChangeFrameStep from {f} to {t}"
+  | .RemoveFrameStep sid => s!"State.RemoveFrameStep {sid}"
+  | .BackRef b f sid =>
+      s!"State.BackRef {b} {if f then "case_insensitive" else ""} => {sid}"
+  | .ByteRange trans =>
+      s!"State.ByteRange {Nat.intAsString trans.start}-{Nat.intAsString trans.end} => {trans.next}"
+  | .SparseTransitions trans =>
+      let lines := String.join (trans.toList |> List.map (fun t =>
+            s!" {Nat.intAsString t.start}-{Nat.intAsString t.end} => {t.next}"))
+      s!"State.SparseTransitions [{lines} ]"
+  | .Look look next =>
+      s!"State.Look {look} => {next}"
+  | .Union alts =>
+      let lines := String.join (alts.toList |> List.map (fun t => s!" {t}"))
+      s!"State.Union [{lines} ]"
+  | .UnionReverse alts =>
+      let lines := String.join (alts.toList |> List.map (fun t => s!" {t}"))
+      s!"State.UnionReverse [{lines} ]"
+  | .BinaryUnion alt1 alt2 => s!"State.BinaryUnion ({alt1}, {alt2})"
+  | .Capture role next pattern_id group slot _ =>
+      s!"State.Capture {role}(pid={pattern_id}, group={group}, slot={slot}) => {next}"
+  | .Match pattern_id => s!"State.Match ({pattern_id})"
+
+end State
+
+instance : ToString $ State n where toString s := Checked.State.toString s
+
+/-- A char oriented Thompson non-deterministic finite automaton (NFA) with n states -/
+structure NFA where
+  /-- number of states -/
+  n : Nat
+  /-- states of the NFA -/
+  states : Array (State n)
+  /-- capture groups which may match with a empty string -/
+  groups : Array Nat
+  /-- Array of (slot, group) pairs of captures -/
+  slots : Array Capture.SlotGroup
+  /-- simulate a unanchored prefix by the backtracker -/
+  unanchored_prefix_in_backtrack : Bool
+  /-- assertion that n equals size of states -/
+  isEq : n = states.size
+  /-- slots are valid -/
+  slotsValid : Slots.Valid slots
+
+instance : Inhabited NFA where default := ⟨0, #[], #[], #[], false, rfl, by
+                                           unfold Slots.Valid; and_intros <;> grind⟩
+
+instance {nfa : NFA} : Coe (Fin nfa.n) (Fin (Array.size nfa.states)) where
+  coe n := Fin.castLE (by simp[nfa.isEq]) n
+
+def toString (nfa : NFA) : String :=
+  let states := Array.mapFinIdx nfa.states (fun i s _ => (i, s))
+  let states := String.join (states.toList |> List.map (fun (i, s) =>
+      let iv := String.mk (Nat.toDigits 10 i)
+      "\n  " ++ iv ++ ": " ++ s.toString))
+  s!"states {states}\nslots {nfa.slots}"
+
+instance : ToString NFA where
+  toString := Checked.toString
+
+end Checked
+
+private def toFin? (i n : Nat) : Option $ Fin n :=
+  if h : i < n then some ⟨i, h⟩ else none
+
+private def toCkeckedTransition? (t : Unchecked.Transition) (n : Nat)
+    : Option $ Checked.Transition n :=
+  if h : t.next < n
+  then some $ ⟨t.start.toFin, t.end.toFin, ⟨t.next, h⟩⟩
+  else none
+
+def toCkeckedState (s : Unchecked.State) (n : Nat) (h : Unchecked.State.nextOf s < n)
+    : Checked.State n :=
+  match s with
+  | .Empty next => Checked.State.Empty ⟨next, by
+    simp [Unchecked.State.nextOf] at h; exact h⟩
+  | .NextChar offset next => Checked.State.NextChar offset ⟨next, by
+    simp [Unchecked.State.nextOf] at h; exact h⟩
+  | .Fail => Checked.State.Fail
+  | .Eat (.Until s) next => Checked.State.Eat
+      (.Until ⟨s, by simp [Unchecked.State.nextOf] at h; simp [Nat.max_lt.mp h]⟩)
+      ⟨next, by simp [Unchecked.State.nextOf] at h; simp [Nat.max_lt.mp h]⟩
+  | .Eat (.ToLast s) next => Checked.State.Eat
+      (.ToLast ⟨s, by simp [Unchecked.State.nextOf] at h; simp [Nat.max_lt.mp h]⟩)
+      ⟨next, by simp [Unchecked.State.nextOf] at h; simp [Nat.max_lt.mp h]⟩
+  | .ChangeFrameStep f t => Checked.State.ChangeFrameStep
+      ⟨f, by simp [Unchecked.State.nextOf] at h; simp [Nat.max_lt.mp h]⟩
+      ⟨t, by simp [Unchecked.State.nextOf] at h; simp [Nat.max_lt.mp h]⟩
+  | .RemoveFrameStep t => Checked.State.RemoveFrameStep
+      ⟨t, by simp [Unchecked.State.nextOf] at h; exact h⟩
+  | .BackRef b f sid => Checked.State.BackRef b f
+      ⟨sid, by simp [Unchecked.State.nextOf] at h; exact h⟩
+  | .ByteRange ⟨start, «end», next⟩ => Checked.State.ByteRange ⟨start.toNat, «end».toNat,
+          ⟨next, by simp [Unchecked.State.nextOf] at h; exact h⟩⟩
+  | .SparseTransitions trans => Checked.State.SparseTransitions
+      (trans.attach |> Array.map (fun ⟨t, h'⟩ => ⟨t.start.toNat, t.end.toNat, ⟨t.next, by
+        simp [Unchecked.State.nextOf] at h
+        let f : Unchecked.Transition → Nat := fun x => x.next
+        have := List.maxD_of_map_all_lt f h (by
+          intro a ha
+          exact List.mem_map_of_mem ha) t (Array.Mem.val h')
+        simp_all +zetaDelta⟩⟩))
+  | .Look look next => Checked.State.Look look ⟨next, by
+      simp [Unchecked.State.nextOf] at h; exact h⟩
+  | .Union alts => Checked.State.Union (alts.attach |> Array.map
+      (fun ⟨alt, h'⟩ => ⟨alt, by
+        simp [Unchecked.State.nextOf] at h
+        exact List.maxD_all_lt_of_lt h alt (Array.Mem.val h')⟩))
+  | .UnionReverse alts => Checked.State.UnionReverse (alts.attach |> Array.map
+      (fun ⟨alt, h'⟩ => ⟨alt, by
+        simp [Unchecked.State.nextOf] at h
+        exact List.maxD_all_lt_of_lt h alt (Array.Mem.val h')⟩))
+  | .Capture role next pattern_id group slot isValid => Checked.State.Capture role
+          ⟨next, by simp [Unchecked.State.nextOf] at h; exact h⟩ pattern_id group slot isValid
+  | .BinaryUnion alt1 alt2 => Checked.State.BinaryUnion
+      ⟨alt1, by simp [Unchecked.State.nextOf] at h; simp [Nat.max_lt.mp h]⟩
+      ⟨alt2, by simp [Unchecked.State.nextOf] at h; simp [Nat.max_lt.mp h]⟩
+  | .Match pattern_id => Checked.State.Match pattern_id
+
+def toFun (states : Array Unchecked.State) (h : ∀ (i : Nat) _, states[i].nextOf < states.size)
+    : { x // x ∈ states } → Checked.State states.size :=
+  have nextOf_lt_of_mem (s : { x // x ∈ states }) : s.val.nextOf < states.size := by
+    have ⟨i, ⟨hlt, _⟩⟩ := Array.getElem_of_mem s.property
+    have := h i hlt
+    simp_all
+  fun s => toCkeckedState s states.size (nextOf_lt_of_mem s)
