Regex/NFA/Lemmas.lean
@@ -1,0 +1,150 @@
+import Batteries.Data.Fin.Basic
+import Regex.Utils
+import Regex.Data.List.Lemmas
+import Regex.Data.Array.Basic
+import Regex.Data.Array.Lemmas
+import Regex.NFA.Basic
+
+namespace NFA
+
+theorem SlotsValidOfRangeMap (slots : Array Capture.SlotGroup)
+  (h : (List.range slots.size).map (fun i => (i, i.div 2)) = slots.toList)
+    : Slots.Valid slots := by
+  simp
+  and_intros
+  · intros
+    expose_names
+    have hMem (a : Capture.SlotGroup) (h : a ∈ (List.range slots.size).map (fun i => (i, i.div 2)))
+        : a.2 = a.1.div 2 := by
+      grind
+    have := hMem (a, b) (by grind)
+    simp_all
+    rw [Nat.mul_comm]
+    have := @Nat.div_add_mod a 2
+    rw [h_2] at this
+    exact id (Eq.symm this)
+  · intros
+    expose_names
+    have hMem (a : Capture.SlotGroup) (h : a ∈ (List.range slots.size).map (fun i => (i, i.div 2)))
+        : a.2 = a.1.div 2 := by
+      grind
+    have := hMem (a, b) (by grind)
+    simp_all
+    rw [Nat.mul_comm]
+    have := @Nat.div_add_mod a 2
+    rw [h_2] at this
+    exact id (Eq.symm this)
+  · intros
+    expose_names
+    exact ⟨a - 1, ⟨b, by
+    and_intros
+    · have : (a, b) ∈ (List.range slots.size).map (fun i => (i, i.div 2)) := by grind
+      have h : b = (a - 1).div 2 := by
+        rw [h_2]
+        exact Eq.symm (@Nat.div_eq_of_eq_mul_left 2 (b * 2) b (by grind) rfl)
+      have hMem (a : Capture.SlotGroup) (h : a.1 < slots.size ∧ a.2 = a.1.div 2)
+          : a ∈ (List.range slots.size).map (fun i => (i, i.div 2)) := by
+        grind
+      have := hMem (a - 1, b) (And.intro (by grind) h)
+      grind
+    · rfl
+    · grind⟩⟩
+
+instance instLEProdNat : LE Capture.SlotGroup where le := Prod.Lex (· < ·) (· ≤ ·)
+instance instLTProdNat : LT Capture.SlotGroup where lt := Prod.Lex (· < ·) (· < ·)
+
+private theorem mem_toSlots_capture_exists (captures : Array NFA.Capture) (slots : Array Capture.SlotGroup)
+  (h : slots = NFA.Capture.toSlots captures)
+    : ∀ slot ∈ slots, ∃ capture : NFA.Capture, capture ∈ captures ∧ NFA.Capture.toSlots.f capture = slot := by
+  unfold NFA.Capture.toSlots at h
+  simp at h
+  generalize hf : (Array.map NFA.Capture.toSlots.f captures) = filtered at h
+  generalize hs : (filtered.mergeSort NFA.Capture.toSlots.le) = sorted at h
+  intro slot hSlot
+  rw [h] at hSlot
+  have hMemSorted := (Array.mem_unique sorted).mp hSlot
+  rw [← hs] at hMemSorted
+  have hMemFiltered := (Array.mem_mergeSort filtered NFA.Capture.toSlots.le).mp hMemSorted
+  rw [← hf] at hMemFiltered
+  have ⟨state, ⟨hmem, heq⟩⟩ := Array.mem_map.mp hMemFiltered
+  exact ⟨state, by simp [*]⟩
+
+private theorem mem_toSlots_slot_exists (captures : Array NFA.Capture) (slots : Array Capture.SlotGroup)
+  (h : slots = NFA.Capture.toSlots captures)
+    : ∀ capture ∈ captures, (∃ slot ∈ slots, NFA.Capture.toSlots.f capture = slot) := by
+  unfold NFA.Capture.toSlots at h
+  simp at h
+  generalize hf : (Array.map NFA.Capture.toSlots.f captures) = filtered at h
+  generalize hs : (filtered.mergeSort NFA.Capture.toSlots.le) = sorted at h
+  intro capture hCapture
+  let slot := NFA.Capture.toSlots.f capture
+  let hSlot : slot = NFA.Capture.toSlots.f capture := by simp +zetaDelta
+  exact ⟨slot, by
+    have hMemMap := (@Array.mem_map NFA.Capture Capture.SlotGroup slot NFA.Capture.toSlots.f captures).mpr
+                        ⟨capture, And.intro hCapture rfl⟩
+    rw [hf] at hMemMap
+    have hMemSorted := (Array.mem_mergeSort filtered NFA.Capture.toSlots.le).mpr hMemMap
+    rw [hs] at hMemSorted
+    have hMemUnique := (Array.mem_unique sorted).mpr hMemSorted
+    rw [← h] at hMemUnique
+    simp_all⟩
+
+private theorem slotsAreValid_of_slot_mod_eq_0
+  (captures : Array NFA.Capture) (slots : Array Capture.SlotGroup)
+  (hmem : ∀ (slot : Capture.SlotGroup), slot ∈ slots
+          → ∃ capture, capture ∈ captures ∧ NFA.Capture.toSlots.f capture = slot)
+    : ∀ (slot : { slot // slot ∈ slots ∧ slot.fst % 2 = 0 }), slot.val.fst = slot.val.snd * 2 := by
+  intro ⟨s, hs⟩
+  have ⟨capture, hi⟩ := hmem s hs.left
+  unfold NFA.Capture.toSlots.f at hi
+  have hIsValid := capture.isValid
+  simp at hIsValid
+  split at hIsValid
+  · grind
+  · have : s.fst % 2 = 1 := by grind
+    have : s.fst % 2 = 0 := by grind
+    simp_all
+
+private theorem slotsAreValid_of_slot_mod_eq_1
+  (captures : Array NFA.Capture) (slots : Array Capture.SlotGroup)
+  (hmem : ∀ (slot : Capture.SlotGroup), slot ∈ slots
+          → ∃ capture, capture ∈ captures ∧ NFA.Capture.toSlots.f capture = slot)
+    : ∀ (slot : { slot // slot ∈ slots ∧ slot.fst % 2 = 1 }), slot.val.fst = slot.val.snd * 2 + 1 := by
+  intro ⟨s, hs⟩
+  have ⟨capture, hi⟩ := hmem s hs.left
+  unfold NFA.Capture.toSlots.f at hi
+  have hIsValid := capture.isValid
+  simp at hIsValid
+  split at hIsValid <;> grind
+
+private theorem slotsAreValid_if_exists
+  (captures : Array NFA.Capture) (h : NFA.Capture.valid captures)
+  (slots : Array Capture.SlotGroup) (heq : NFA.Capture.toSlots captures = slots)
+  (hmem : ∀ (slot : Capture.SlotGroup), slot ∈ slots
+          → ∃ capture, capture ∈ captures ∧ NFA.Capture.toSlots.f capture = slot)
+    : ∀ (slot : { slot // slot ∈ slots ∧ slot.fst = slot.snd * 2 + 1 }),
+      ∃ slot', slot' ∈ slots ∧ slot.val.snd = slot'.snd ∧ slot'.fst = slot'.snd * 2 := by
+  intro ⟨s, hs⟩
+  have ⟨capture, hCapture⟩ := hmem s hs.left
+  unfold NFA.Capture.valid at h
+  unfold NFA.Capture.toSlots.f at hCapture
+  have hIsValid := capture.isValid
+  simp at hIsValid
+  split at hIsValid; · grind
+  have ⟨capture', hCapture'⟩ := h.right.right ⟨capture, by simp_all⟩
+  have ⟨s', hs'⟩ := mem_toSlots_slot_exists captures slots heq.symm capture' hCapture'.left
+  exact ⟨s', by
+    and_intros
+    simp_all
+    all_goals simp [Capture.toSlots.f] at hs' <;> simp_all <;> grind⟩
+
+theorem toSlots_valid (captures : Array NFA.Capture)
+  (h : NFA.Capture.valid captures)
+    : Slots.Valid (NFA.Capture.toSlots captures) := by
+  generalize hs : NFA.Capture.toSlots captures = slots
+  unfold Slots.Valid
+  have hmem := mem_toSlots_capture_exists captures slots hs.symm
+  and_intros
+  · exact slotsAreValid_of_slot_mod_eq_0 captures slots hmem
+  · exact slotsAreValid_of_slot_mod_eq_1 captures slots hmem
+  · exact slotsAreValid_if_exists captures h slots hs hmem
